Start handling properties

Veir/IR/Buffed/Layout.lean
@@ -90,8 +90,7 @@ end BlockOperand
 namespace Operation
 variable [HasOpInfo OpInfo] (op : OperationPtr) (ctx : IRContext OpInfo)
 
--- Add this info to the typeclasses
-def propertySize (_opCode : OpInfo) : UInt64 := 8
+def propertySize (opCode : OpInfo) : UInt64 := HasDialectOpInfo.propertySize opCode
 @[inline] abbrev opInfoSize : Nat := 8
 
 namespace Sizes
